theories/zoo_saturn/spsc_bqueue__opaque.v
@@ -2,6 +2,7 @@ From zoo_saturn Require Import
   spsc_bqueue__code.
 
 #[global] Opaque spsc_bqueue_create.
+#[global] Opaque spsc_bqueue_capacity.
 #[global] Opaque spsc_bqueue_size.
 #[global] Opaque spsc_bqueue_is_empty.
 #[global] Opaque spsc_bqueue_push.
